Redefine FiniteProj as a sigma type
Instead of

  Definition FiniteProj (A B : Type) (p : A -> B) : Prop :=
    exists l : list A, FullProj p l.

we now have

  Definition FiniteProj (A B : Type) (p : A -> B) : Type :=
    { l : list A | FullProj p l }.

The point is that computations can now destruct a FiniteProj to get
the list witnessing its finiteness.

The main use is in fin_mod. Now, if you have an object of
type (fin_mod f), then a computation can extract the finite list of
domain elements.

The biggest resulting changes are in Perm.v, where we can now actually
define the inverse map (before, we had to destruct the exist Prop, so
could only assert that the inverse map existed.

FinSet/FPCard.v
@@ -263,37 +263,32 @@ Section inj_endo.
 
   Variable a0 : A.
 
-  Local Definition g {l} (fullH : FullProj p l) : nat_map p p :=
+  Definition inj_endo_inv {l} (fullH : FullProj p l) : nat_map p p :=
     surj_nat_map_right_inverse decB decB a0 inj_endo_is_surj fullH.
 
-  Local Lemma g_is_right_inv
+  Local Lemma inj_endo_inv_right
         {l} (fullH : FullProj p l)
-    : forall a, nm_bot (nat_map_comp_h (g fullH) f) (p a) = p a.
+    : forall a, nm_bot (nat_map_comp_h (inj_endo_inv fullH) f) (p a) = p a.
   Proof.
     apply (surj_map_is_invertible decB decB a0 inj_endo_is_surj fullH).
   Qed.
 
-  Local Lemma g_is_left_inv
+  Local Lemma inj_endo_inv_left
         {l} (fullH : FullProj p l)
-    : forall a, nm_bot (nat_map_comp_h f (g fullH)) (p a) = p a.
+    : forall a, nm_bot (nat_map_comp_h f (inj_endo_inv fullH)) (p a) = p a.
   Proof.
     intro a.
     unfold inj_nat_map in injH.
-    pose proof (g_is_right_inv fullH (nm_top f a)) as gfH.
-    rewrite nat_map_nat in gfH.
-    rewrite <- nm_bot_comp_h in gfH.
-    rewrite nm_comp_h_assoc_bot in gfH.
-    rewrite nm_bot_comp_h in gfH.
-    rewrite <- nat_map_nat in gfH.
-    rewrite <- nat_map_nat.
-    exact (injH _ _ gfH).
+    pose proof (inj_endo_inv_right fullH (nm_top f a)) as gfH; revert gfH.
+    rewrite nat_map_nat,
+            <- nm_bot_comp_h, nm_comp_h_assoc_bot, nm_bot_comp_h,
+            <- nat_map_nat.
+    apply injH.
   Qed.
 
-  Lemma inj_endo_is_invertible : exists h : nat_map p p, inv_bottom f h.
+  Lemma inj_endo_is_invertible : inv_bottom f (inj_endo_inv (proj2_sig finH)).
   Proof.
-    destruct finH as [ l fullH ].
-    exists (g fullH).
-    constructor; auto using g_is_right_inv, g_is_left_inv.
+    split; auto using inj_endo_inv_right, inj_endo_inv_left.
   Qed.
 End inj_endo.
 
